utp/utp_procedure.thy
@@ -7,34 +7,34 @@ begin
 type_synonym ('a, '\<alpha>) uproc = "'a \<Rightarrow> '\<alpha> hrelation"
 
 definition 
-  val_parm :: "('a::two, '\<alpha>) lvar \<Rightarrow> (('a, '\<alpha>) uvar \<Rightarrow> '\<alpha> hrelation) 
-               \<Rightarrow> (('a, '\<alpha>) uexpr, '\<alpha>) uproc"
-where "val_parm x P = (\<lambda> v. (var x \<bullet> (x := v ;; P x)))"
+  val_parm :: "('\<T> \<times> '\<alpha>) itself \<Rightarrow> ('a::two, '\<beta>) lvar \<Rightarrow> (('a, '\<beta>) uvar \<Rightarrow> '\<alpha> hrelation) 
+               \<Rightarrow> (('a, '\<beta>) uexpr, '\<alpha>) uproc"
+where "val_parm T x P = (\<lambda> v. (var\<^bsub>T\<^esub> x \<bullet> (x ::=\<^bsub>T\<^esub> v ;; P x)))"
 
 definition 
-  val_parm_comp :: "('a::two, '\<alpha>) lvar \<Rightarrow> (('a, '\<alpha>) uvar \<Rightarrow> ('b, '\<alpha>) uproc) 
-               \<Rightarrow> (('a, '\<alpha>) uexpr \<times> 'b, '\<alpha>) uproc"
-where "val_parm_comp x P = (\<lambda> (u, v). (var x \<bullet> (x := u ;; P x v)))"
+  val_parm_comp :: "('\<T> \<times> '\<alpha>) itself \<Rightarrow> ('a::two, '\<beta>) lvar \<Rightarrow> (('a, '\<beta>) uvar \<Rightarrow> ('b, '\<alpha>) uproc) 
+               \<Rightarrow> (('a, '\<beta>) uexpr \<times> 'b, '\<alpha>) uproc"
+where "val_parm_comp T x P = (\<lambda> (u, v). (var\<^bsub>T\<^esub> x \<bullet> (x ::=\<^bsub>T\<^esub> u ;; P x v)))"
 
 definition 
-  res_parm :: "('a::two, '\<alpha>) lvar \<Rightarrow> (('a, '\<alpha>) uvar \<Rightarrow> '\<alpha> hrelation) 
-               \<Rightarrow> (('a, '\<alpha>) uvar, '\<alpha>) uproc"
-where "res_parm x P = (\<lambda> y. (var x \<bullet> (P x ;; y := &x)))"
+  res_parm :: "('\<T> \<times> '\<alpha>) itself \<Rightarrow> ('a::two, '\<beta>) lvar \<Rightarrow> (('a, '\<beta>) uvar \<Rightarrow> '\<alpha> hrelation) 
+               \<Rightarrow> (('a, '\<beta>) uvar, '\<alpha>) uproc"
+where "res_parm T x P = (\<lambda> y. (var\<^bsub>T\<^esub> x \<bullet> (P x ;; y ::=\<^bsub>T\<^esub> &x)))"
 
 definition 
-  res_parm_comp :: "('a::two, '\<alpha>) lvar \<Rightarrow> (('a, '\<alpha>) uvar \<Rightarrow> ('b, '\<alpha>) uproc) 
-               \<Rightarrow> (('a, '\<alpha>) uvar \<times> 'b, '\<alpha>) uproc"
-where "res_parm_comp x P = (\<lambda> (u, v). (var x \<bullet> (P x v ;; u := &x)))"
+  res_parm_comp :: "('\<T> \<times> '\<alpha>) itself \<Rightarrow> ('a::two, '\<beta>) lvar \<Rightarrow> (('a, '\<beta>) uvar \<Rightarrow> ('b, '\<alpha>) uproc) 
+               \<Rightarrow> (('a, '\<beta>) uvar \<times> 'b, '\<alpha>) uproc"
+where "res_parm_comp T x P = (\<lambda> (u, v). (var\<^bsub>T\<^esub> x \<bullet> (P x v ;; u ::=\<^bsub>T\<^esub> &x)))"
 
 definition
-  vres_parm :: "('a::two, '\<alpha>) lvar \<Rightarrow> (('a, '\<alpha>) uvar \<Rightarrow> '\<alpha> hrelation) 
-               \<Rightarrow> (('a, '\<alpha>) uvar, '\<alpha>) uproc"
-where "vres_parm x P = (\<lambda> y. (var x \<bullet> (x := &y ;; P x ;; y := &x)))"
+  vres_parm :: "('\<T> \<times> '\<alpha>) itself \<Rightarrow> ('a::two, '\<beta>) lvar \<Rightarrow> (('a, '\<beta>) uvar \<Rightarrow> '\<alpha> hrelation) 
+               \<Rightarrow> (('a, '\<beta>) uvar, '\<alpha>) uproc"
+where "vres_parm T x P = (\<lambda> y. (var\<^bsub>T\<^esub> x \<bullet> (x ::=\<^bsub>T\<^esub> &y ;; P x ;; y ::=\<^bsub>T\<^esub> &x)))"
 
 definition 
-  vres_parm_comp :: "('a::two, '\<alpha>) lvar \<Rightarrow> (('a, '\<alpha>) uvar \<Rightarrow> ('b, '\<alpha>) uproc) 
-               \<Rightarrow> (('a, '\<alpha>) uvar \<times> 'b, '\<alpha>) uproc"
-where "vres_parm_comp x P = (\<lambda> (u, v). (var x \<bullet> (x := &u ;; P x v ;; u := &x)))"
+  vres_parm_comp :: "('\<T> \<times> '\<alpha>) itself \<Rightarrow> ('a::two, '\<beta>) lvar \<Rightarrow> (('a, '\<beta>) uvar \<Rightarrow> ('b, '\<alpha>) uproc) 
+               \<Rightarrow> (('a, '\<beta>) uvar \<times> 'b, '\<alpha>) uproc"
+where "vres_parm_comp T x P = (\<lambda> (u, v). (var\<^bsub>T\<^esub> x \<bullet> (x ::=\<^bsub>T\<^esub> &u ;; P x v ;; u ::=\<^bsub>T\<^esub> &x)))"
 
 nonterminal parm and parm_list
 
@@ -44,39 +44,45 @@ syntax
   "_parm_list"    :: "parm \<Rightarrow> parm_list \<Rightarrow> parm_list" ("_ ,/ _")
   "_tparm"        :: "parm_list \<Rightarrow> logic" ("_")
   "_proc_block"   :: "parm_list \<Rightarrow> logic \<Rightarrow> ('a, '\<alpha>) uproc" ("_ \<bullet>/ _" [0,10] 10)
-  "_val_parm"     :: "id \<Rightarrow> parm" ("val _" [999] 999)
-  "_val_parm_ty"  :: "id \<Rightarrow> type \<Rightarrow> parm" ("val _ :: _")
-  "_res_parm"     :: "id \<Rightarrow> parm" ("res _" [999] 999)
-  "_res_parm_ty"  :: "id \<Rightarrow> type \<Rightarrow> parm" ("res _ :: _")
-  "_vres_parm"    :: "id \<Rightarrow> parm" ("vres _" [999] 999)
-  "_vres_parm_ty" :: "id \<Rightarrow> type \<Rightarrow> parm" ("vres _ :: _" [0,999] 999)
+  "_val_parm"     :: "logic \<Rightarrow> id \<Rightarrow> parm" ("val\<index> _" [999] 999)
+  "_val_parm_ty"  :: "logic \<Rightarrow> id \<Rightarrow> type \<Rightarrow> parm" ("val\<index> _ :: _")
+  "_res_parm"     :: "logic \<Rightarrow> id \<Rightarrow> parm" ("res\<index> _" [999] 999)
+  "_res_parm_ty"  :: "logic \<Rightarrow> id \<Rightarrow> type \<Rightarrow> parm" ("res\<index> _ :: _")
+  "_vres_parm"    :: "logic \<Rightarrow> id \<Rightarrow> parm" ("vres\<index> _" [999] 999)
+  "_vres_parm_ty" :: "logic \<Rightarrow> id \<Rightarrow> type \<Rightarrow> parm" ("vres\<index> _ :: _" [0,999] 999)
 
 translations
   (* Parse translations for value parameters *)
-  "_proc_block (_parm (_val_parm x)) P" => "CONST val_parm <x>\<^sub>d (\<lambda> x. P)"
-  "_proc_block (_parm (_val_parm_ty x a)) P" => "CONST val_parm <x>\<^sub>d (_abs (_constrain x (_uvar_ty a)) P)"
-  "_proc_block (_parm_list (_val_parm_ty x a) ps) P" 
-  => "CONST val_parm_comp <x>\<^sub>d (_abs (_constrain x (_uvar_ty a)) (_proc_block ps P))"
-  "_proc_block (_parm_list (_val_parm x) ps) P" 
-  => "CONST val_parm_comp <x>\<^sub>d (\<lambda> x. (_proc_block ps P))"
+  "_proc_block (_parm (_val_parm T x)) P" => "CONST val_parm T <x>\<^sub>d (\<lambda> x. P)"
+  "_proc_block (_parm (_val_parm_ty T x a)) P" => "CONST val_parm T <x>\<^sub>d (_abs (_constrain x (_uvar_ty a)) P)"
+  "_proc_block (_parm_list (_val_parm_ty T x a) ps) P" 
+  => "CONST val_parm_comp T <x>\<^sub>d (_abs (_constrain x (_uvar_ty a)) (_proc_block ps P))"
+  "_proc_block (_parm_list (_val_parm T x) ps) P" 
+  => "CONST val_parm_comp T <x>\<^sub>d (\<lambda> x. (_proc_block ps P))"
   (* Parse translations for result parameters *)
-  "_proc_block (_parm (_res_parm x)) P" => "CONST res_parm <x>\<^sub>d (\<lambda> x. P)"
-  "_proc_block (_parm (_res_parm_ty x a)) P" => "CONST res_parm <x>\<^sub>d (_abs (_constrain x (_uvar_ty a)) P)"
-  "_proc_block (_parm_list (_res_parm_ty x a) ps) P" 
-  => "CONST res_parm_comp <x>\<^sub>d (_abs (_constrain x (_uvar_ty a)) (_proc_block ps P))"
-  "_proc_block (_parm_list (_res_parm x) ps) P" 
-  => "CONST res_parm_comp <x>\<^sub>d (\<lambda> x. (_proc_block ps P))"
+  "_proc_block (_parm (_res_parm T x)) P" => "CONST res_parm T <x>\<^sub>d (\<lambda> x. P)"
+  "_proc_block (_parm (_res_parm_ty T x a)) P" => "CONST res_parm T <x>\<^sub>d (_abs (_constrain x (_uvar_ty a)) P)"
+  "_proc_block (_parm_list (_res_parm_ty T x a) ps) P" 
+  => "CONST res_parm_comp T <x>\<^sub>d (_abs (_constrain x (_uvar_ty a)) (_proc_block ps P))"
+  "_proc_block (_parm_list (_res_parm T x) ps) P" 
+  => "CONST res_parm_comp T <x>\<^sub>d (\<lambda> x. (_proc_block ps P))"
   (* Parse translations for value-result parameters *)
-  "_proc_block (_parm (_vres_parm x)) P" => "CONST vres_parm <x>\<^sub>d (\<lambda> x. P)"
-  "_proc_block (_parm (_vres_parm_ty x a)) P" => "CONST vres_parm <x>\<^sub>d (_abs (_constrain x (_uvar_ty a)) P)"
-  "_proc_block (_parm_list (_vres_parm_ty x a) ps) P" 
-  => "CONST vres_parm_comp <x>\<^sub>d (_abs (_constrain x (_uvar_ty a)) (_proc_block ps P))"
-  "_proc_block (_parm_list (_res_parm x) ps) P" 
-  => "CONST vres_parm_comp <x>\<^sub>d (\<lambda> x. (_proc_block ps P))"
+  "_proc_block (_parm (_vres_parm T x)) P" => "CONST vres_parm T <x>\<^sub>d (\<lambda> x. P)"
+  "_proc_block (_parm (_vres_parm_ty T x a)) P" => "CONST vres_parm T <x>\<^sub>d (_abs (_constrain x (_uvar_ty a)) P)"
+  "_proc_block (_parm_list (_vres_parm_ty T x a) ps) P" 
+  => "CONST vres_parm_comp T <x>\<^sub>d (_abs (_constrain x (_uvar_ty a)) (_proc_block ps P))"
+  "_proc_block (_parm_list (_res_parm T x) ps) P" 
+  => "CONST vres_parm_comp T <x>\<^sub>d (\<lambda> x. (_proc_block ps P))"
+
+(*
+context utp_local_var
+begin
+
+declare [[show_types]]
 
 lemma val_parm_apply [simp]: 
-  "val_parm x P v = (var x \<bullet> (P x)\<lbrakk>\<lceil>v\<rceil>\<^sub></$x\<rbrakk>)"
-  by (simp add: assigns_r_comp subst_lift_id subst_lift_upd val_parm_def)
+  "val_parm \<T> x P v = (var x \<bullet> (P x)\<lbrakk>\<lceil>v\<rceil>\<^sub></$x\<rbrakk>)"
+ apply (simp add: assigns_r_comp  subst_lift_upd val_parm_def)
 
 lemma val_parm_comp_apply:
   "(val_parm_comp x P) (u, v) = (var x \<bullet> (P x v)\<lbrakk>\<lceil>u\<rceil>\<^sub></$x\<rbrakk>)"
@@ -97,6 +103,7 @@ lemma vres_parm_apply [simp]:
 lemma vres_parm_comp_apply [simp]: 
   "(vres_parm_comp x P) (u, v) = (var x \<bullet> x := &u ;; P x v ;; u := &x)"
   by (simp add: vres_parm_comp_def)
+*)
 
 text {* Instantiate vstore for design alphabets *}
 
@@ -106,5 +113,6 @@ begin
 instance
   by (intro_classes, auto simp add: vstore_lens_alpha_d_ext_def comp_vwb_lens)
 end
+
 
 end
